src/cbor/pulse/raw/CBOR.Pulse.API.Det.Common.fst
@@ -1549,3 +1549,30 @@ fn cbor_det_map_get (_: unit)
   }
 }
 ```
+
+module Copy = CBOR.Pulse.Raw.Copy
+
+let freeable = Copy.freeable
+
+let get_cbor_from_freeable x = Copy.Mkfreeable_cbor?.cbor x
+
+```pulse
+  fn cbor_copy (_: unit)
+: cbor_copy_t u#0 u#0 #_ #_ cbor_det_match freeable get_cbor_from_freeable
+=
+  (c: _)
+  (#p: _)
+  (#v: _)
+{
+  unfold (cbor_det_match p c v);
+  let res = Copy.cbor_copy c;
+  fold (cbor_det_match p c v);
+  Trade.rewrite_with_trade
+    (Raw.cbor_match 1.0R res.cbor (SpecRaw.mk_det_raw_cbor v))
+    (cbor_det_match 1.0R (get_cbor_from_freeable res) v);
+  Trade.trans _ _ (freeable res);
+  res
+}
+```
+
+let cbor_free _ x = Copy.cbor_free x
