src/cbor/pulse/CBOR.Pulse.API.Det.Type.fsti
@@ -11,3 +11,6 @@ val cbor_det_map_iterator_t: Type0
 
 inline_for_extraction noextract [@@noextract_to "krml"]
 val dummy_cbor_det_t (_: unit) : cbor_det_t
+
+[@@CAbstractStruct]
+val freeable_cbor_det_t: Type0
